games/HComp.v
@@ -1,7 +1,10 @@
 Require Import ATS.
 Require Import MultiChannel.
+Require Import KLR.
 Require Import List.
 
+
+(** * Flat composition *)
 
 (** The flat composition of a family of alternating transition systems
   switches between them with each opponent question, allowing one
@@ -10,6 +13,9 @@ Require Import List.
   remembers what component asked what pending question. *)
 
 Module FComp.
+
+  (** ** Definition *)
+
   Section ATS.
     Context {GA GB : game} {I S K} (α : ats (GA ^ I) (GB ^ I) S K).
 
@@ -23,20 +29,20 @@ Module FComp.
 
     Inductive suspend : state -> pmove GA GB * cont -> Prop :=
       | suspend_q (m : question GA) i s k stk :
-          ATS.suspend α s (Pow.mkp i (inl m), k) ->
-          suspend (s, stk) (inl m, (k, i :: stk))
+          ATS.suspend α s (Pow.mkp i (pq m), k) ->
+          suspend (s, stk) (pq m, (k, i :: stk))
       | suspend_a (m : answer GB) i s k stk :
-          ATS.suspend α s (Pow.mkp i (inr m), k) ->
-          suspend (s, stk) (inr m, (k, stk)).
+          ATS.suspend α s (Pow.mkp i (pa m), k) ->
+          suspend (s, stk) (pa m, (k, stk)).
 
     Inductive resume : cont -> omove GA GB -> state -> Prop :=
       | resume_q (m : question GB) i s k stk :
           (forall j, ATS.refuse α k (j, m)) ->
-          ATS.resume α k (Pow.mko i (inr m)) s ->
-          resume (k, stk) (inr m) (s, stk)
+          ATS.resume α k (Pow.mko i (oq m)) s ->
+          resume (k, stk) (oq m) (s, stk)
       | resume_a (m : answer GA) i s k stk :
-          ATS.resume α k (Pow.mko i (inl m)) s ->
-          resume (k, i :: stk) (inl m) (s, stk).
+          ATS.resume α k (Pow.mko i (oa m)) s ->
+          resume (k, i :: stk) (oa m) (s, stk).
 
     Inductive refuse : cont -> oqmove GA GB -> Prop :=
       | refuse_intro (m : question GB) k stk :
@@ -47,6 +53,200 @@ Module FComp.
       ATS.Build_ats GA GB state cont step suspend resume refuse.
 
   End ATS.
+
+  Arguments state : clear implicits.
+  Arguments cont : clear implicits.
+
+  (** ** Monotonicity *)
+
+  Section SIMREL.
+    Context {I : Type}.
+    Context {GA1 GB1 : game} {S1 K1} (α1 : ats (GA1 ^ I) (GB1 ^ I) S1 K1).
+    Context {GA2 GB2 : game} {S2 K2} (α2 : ats (GA2 ^ I) (GB2 ^ I) S2 K2).
+    Context {GRA : grel GA1 GA2} {GRB : grel GB1 GB2}.
+
+    Definition sum_map {A1 A2} f {B1 B2} g : A1 + B1 -> A2 + B2 :=
+      fun x =>
+        match x with
+          | inl a => inl (f a)
+          | inr b => inr (g b)
+        end.
+
+    Fixpoint wstack (ws : gworld (GRA ^ I) (GRB ^ I)) : list I :=
+      match ws with
+        | inl w :: ws => fst w :: wstack ws
+        | inr w :: ws => wstack ws
+        | nil => nil
+      end.
+
+    Fixpoint wproj (ws : gworld (GRA ^ I) (GRB ^ I)) : gworld GRA GRB :=
+      match ws with
+        | inl w :: ws => inl (snd w) :: wproj ws
+        | inr w :: ws => inr (snd w) :: wproj ws
+        | nil => nil
+      end.
+
+    Inductive state_rel (RS : klr _ S1 S2) : klr _ (state I S1) (state I S2) :=
+      state_rel_intro ws s1 s2 :
+        RS ws s1 s2 ->
+        state_rel RS (wproj ws) (s1, wstack ws) (s2, wstack ws).
+
+    Inductive cont_rel (RK : klr _ K1 K2) : klr _ (cont I K1) (cont I K2) :=
+      cont_rel_intro ws k1 k2 :
+        RK ws k1 k2 ->
+        cont_rel RK (wproj ws) (k1, wstack ws) (k2, wstack ws).
+  End SIMREL.
+
+  Global Instance step_sim :
+    Monotonic
+      (@step)
+      (forallr GRA, forallr GRB, forallr - @ I, forallr RS, forallr RK,
+        ATS.sim (GRA ^ I) (GRB ^ I) RS RK ++>
+        |= state_rel RS ++> k1 set_le (state_rel RS)).
+  Proof.
+    intros GA1 GA2 GRA GB1 GB2 GRB I S1 S2 RS K1 K2 RK.
+    intros α1 α2 Hα ws s1 s2 Hs s1' Hs1'.
+    destruct Hs1' as [s1 s1' stk Hs1'].
+    inversion Hs as [iws xs1 xs2]; clear Hs; subst.
+    edestruct @ATS.sim_step as (s2' & Hs2' & Hs'); eauto.
+    exists (s2', wstack iws). intuition idtac.
+    - constructor; auto.
+    - constructor; auto.
+  Qed.
+
+  Lemma gacc_inv_pq {GA1 GA2} GRA {GB1 GB2} GRB q1 m2 ws ws' :
+    @gacc GA1 GA2 GRA GB1 GB2 GRB (pm (pq q1), m2) ws ws' ->
+    exists w q2,
+      m2 = pm (pq q2) /\
+      question_rel GRA w q1 q2 /\
+      ws' = inl w :: ws.
+  Proof.
+    intros H.
+    inversion H; clear H; subst;
+    inversion H4; clear H4; subst.
+    eauto.
+  Qed.
+
+  Lemma gacc_inv_pa {GA1 GA2} GRA {GB1 GB2} GRB a1 m2 ws ws' :
+    @gacc GA1 GA2 GRA GB1 GB2 GRB (pm (pa a1), m2) ws ws' ->
+    exists w a2,
+      m2 = pm (pa a2) /\
+      answer_rel GRB w a1 a2 /\
+      ws = inr w :: ws'.
+  Proof.
+    intros H.
+    inversion H; clear H; subst;
+    inversion H4; clear H4; subst.
+    eauto.
+  Qed.
+
+  Global Instance suspend_sim :
+    Monotonic
+      (@suspend)
+      (forallr GRA, forallr GRB, forallr - @ I, forallr RS, forallr RK,
+        ATS.sim (GRA ^ I) (GRB ^ I) RS RK ++>
+        |= state_rel RS ++> k1 set_le (<> * cont_rel RK)).
+  Proof.
+    intros GA1 GA2 GRA GB1 GB2 GRB I S1 S2 RS K1 K2 RK.
+    intros α1 α2 Hα ws mk1 mk2 Hmk mk1' Hmk1'.
+    destruct Hmk1' as [q1 i1 s1 k1 stk H1 | a1 i1 s1 k1 stk H1];
+    inversion Hmk; clear Hmk; subst.
+    - edestruct @ATS.sim_suspend as ([m2 k2] & Hmk2 & Hmk); eauto.
+      destruct Hmk as (ws' & Hws' & Hk). simpl in Hws'. 
+      apply gacc_inv_pq in Hws' as (w & q2 & Hm2 & Hq & Hws'). subst.
+      inversion Hm2; clear Hm2; subst.
+      simpl in Hq. destruct w as [i w].
+      rinversion Hq; clear Hq. destruct H. inversion Hql; clear Hql; subst.
+      eexists (pq b2, (k2, _)). split.
+      + constructor; eauto.
+      + red. eexists (wproj (inl (i1, w) :: ws0)). split.
+        * constructor. constructor. auto.
+        * constructor. auto.
+    - edestruct @ATS.sim_suspend as ([m2 k2] & Hmk2 & Hmk); eauto.
+      destruct Hmk as (ws' & Hws' & Hk). simpl in Hws'. 
+      apply gacc_inv_pa in Hws' as (w & a2 & Hm2 & Ha & Hws). subst.
+      inversion Hm2; clear Hm2; subst.
+      simpl in Ha. destruct w as [i w].
+      rinversion Ha; clear Ha. destruct H. inversion Hal; clear Hal; subst.
+      eexists (pa b2, (k2, _)). split.
+      + econstructor; eauto.
+      + eexists (wproj ws'). split.
+        * constructor. constructor. auto.
+        * simpl. constructor. auto.
+  Qed.
+
+  Global Instance resume_sim :
+    Monotonic
+      (@resume)
+      (forallr GRA, forallr GRB, forallr - @ I, forallr RS, forallr RK,
+       ATS.sim (GRA ^ I) (GRB ^ I) RS RK ++>
+       |= cont_rel RK ++> ([] -> k1 set_le (state_rel RS))).
+  Proof.
+    intros GA1 GA2 GRA GB1 GB2 GRB I S1 S2 RS K1 K2 RK.
+    intros α1 α2 Hα ws k1 k2 Hk m1 m2 ws' Hm s1 Hs1.
+    destruct Hs1 as [q1 i1 s1 k1 stk Hr1 Hs1 | a1 i1 s1 k1 stk Hs1];
+    inversion Hk; clear Hk; subst;
+    inversion Hm; clear Hm; subst.
+    - inversion H4; clear H4; subst.
+      edestruct @ATS.sim_resume as (s2 & Hs2 & Hs); eauto.
+      + instantiate (1 := inr (i1, w0) :: ws0).
+        instantiate (1 := Pow.mko i1 (oq m0)).
+        repeat constructor. simpl. auto.
+      + exists (s2, wstack ws0). split.
+        * econstructor; eauto.
+          intro j. eapply ATS.sim_refuse, Hr1; eauto.
+          instantiate (1 := inr (j, w0) :: ws0).
+          instantiate (1 := j). simpl.
+          repeat constructor; eauto.
+        * change (_ :: _) with (wproj (inr (i1, w0) :: ws0)).
+          change (wstack ws0) with (wstack (inr (i1, w0) :: ws0)).
+          constructor; auto.
+    - inversion H4.
+    - inversion H5.
+    - inversion H5; clear H5; subst.
+      destruct ws0 as [ | [w|w] ws]; inversion H4; clear H4; subst.
+      simpl in H2. inversion H2; clear H2; subst.
+      destruct w as [i w]; cbv [fst snd] in *.
+      edestruct @ATS.sim_resume as (s2 & Hs2 & Hs); eauto.
+      + instantiate (1 := ws).
+        instantiate (1 := Pow.mko i (oa m0)).
+        repeat constructor. simpl. auto.
+      + exists (s2, wstack ws). split.
+        * constructor; auto.
+        * constructor; auto.
+  Qed.
+
+  Global Instance refuse_sim :
+    Monotonic
+      (@refuse)
+      (forallr GRA, forallr GRB, forallr - @ I, forallr RS, forallr RK,
+       ATS.sim (GRA ^ I) (GRB ^ I) RS RK ++>
+       |= cont_rel RK ++> ([] -> k impl)).
+  Proof.
+    intros GA1 GA2 GRA GB1 GB2 GRB I S1 S2 RS K1 K2 RK.
+    intros α1 α2 Hα ws k1 k2 Hk m1 m2 ws' Hm Hm1.
+    destruct Hm1;
+    inversion Hk; clear Hk; subst;
+    inversion Hm; clear Hm; subst;
+    inversion H5; clear H5; subst.
+    constructor. intro i.
+    eapply ATS.sim_refuse, H; eauto.
+    instantiate (1 := inr (i, w0) :: ws0).
+    instantiate (1 := i).
+    repeat constructor; auto.
+  Qed.
+
+  Global Instance of_sim :
+    Monotonic
+      (@of)
+      (forallr GRA, forallr GRB, forallr - @ I, forallr RS, forallr RK,
+       ATS.sim (GRA ^ I) (GRB ^ I) RS RK ++>
+       ATS.sim GRA GRB (state_rel RS) (cont_rel RK)).
+  Proof.
+    intros GA1 GA2 GRA GB1 GB2 GRB I S1 S2 RS K1 K2 RK α1 α2 H.
+    split; simpl; try rauto.
+  Qed.
+
 End FComp.
 
 (** The resolution operator allows a component to interact with itself
@@ -68,30 +268,30 @@ Module Res.
           ATS.step α s s' ->
           step (s, stk) (s', stk)
       | step_q (m : question G) s k s' stk :
-          ATS.suspend α s (inl m, k) ->
-          ATS.resume α k (inr m) s' ->
+          ATS.suspend α s (pq m, k) ->
+          ATS.resume α k (oq m) s' ->
           step (s, stk) (s', true :: stk)
       | step_a (m : answer G) s k s' stk :
-          ATS.suspend α s (inr m, k) ->
-          ATS.resume α k (inl m) s' ->
+          ATS.suspend α s (pa m, k) ->
+          ATS.resume α k (oa m) s' ->
           step (s, true :: stk) (s', stk).
 
     Inductive suspend : state -> pmove G G * cont -> Prop :=
       | suspend_q (m : question G) s k stk :
-          ATS.suspend α s (inl m, k) ->
+          ATS.suspend α s (pq m, k) ->
           ATS.refuse α k m ->
-          suspend (s, stk) (inl m, (k, stk))
+          suspend (s, stk) (pq m, (k, stk))
       | suspend_a (m : answer G) s k stk :
-          ATS.suspend α s (inr m, k) ->
-          suspend (s, false :: stk) (inr m, (k, stk)).
+          ATS.suspend α s (pa m, k) ->
+          suspend (s, false :: stk) (pa m, (k, stk)).
 
     Inductive resume : cont -> omove G G -> state -> Prop :=
       | resume_q m k s stk :
-          ATS.resume α k (inr m) s ->
-          resume (k, stk) (inr m) (s, false :: stk)
+          ATS.resume α k (oq m) s ->
+          resume (k, stk) (oq m) (s, false :: stk)
       | resume_a m k s stk :
-          ATS.resume α k (inl m) s ->
-          resume (k, stk) (inl m) (s, stk).
+          ATS.resume α k (oa m) s ->
+          resume (k, stk) (oa m) (s, stk).
 
     Inductive refuse : cont -> oqmove G G -> Prop :=
       | refuse_intro k m stk :
